src/generatedproof/controllers/replicaset.v
@@ -6,6 +6,7 @@ Require Export New.generatedproof.k8s_io.api.core.v1.
 Require Export New.generatedproof.k8s_io.apimachinery.pkg.api.errors.
 Require Export New.generatedproof.k8s_io.apimachinery.pkg.apis.meta.v1.
 Require Export New.generatedproof.k8s_io.kubernetes.pkg.controller.
+Require Export New.generatedproof.kubernetes_model.apimodel.
 Require Export New.golang.theory.
 Require Export New.code.controllers.replicaset.
 
